{
 "cells": [
  {
   "cell_type": "markdown",
   "id": "11c2c5b6",
   "metadata": {},
   "source": [
    "# Assignment Lecture 1\n",
    "\n"
   ]
  },
  {
   "cell_type": "markdown",
   "id": "aff2b667",
   "metadata": {},
   "source": [
    "Garcia, James Matthew C. <br> BSCS - 1 <br>\n",
    "***"
   ]
  },
  {
   "cell_type": "markdown",
   "id": "ebbedbdc",
   "metadata": {},
   "source": [
    "1. Recall the definition of a rational number, denoted as $\\mathbb{Q}$. Prove that the Euler's number $e = \\Sigma_{k=0}^\\infty \\frac{1}{k!} \\notin \\mathbb{Q}$. A factorial is defined as $k! = (k)(k-1)(k-2)(k-3)..., \\forall k \\in \\mathbb{Z}^+$, note that $0! = 1$. Furthermore, a sum notation $\\Sigma_{k=0}^\\infty k = 0+ 1 + 2 + 3 +....+...$"
   ]
  },
  {
   "cell_type": "markdown",
   "id": "9738db87",
   "metadata": {},
   "source": [
    "**Solution**: <br>\n",
    "Proof by Contradiction: <br><br>\n",
    "Let $p\\in \\mathbb{Z}$ and $q \\in \\mathbb{N}$ such that $e = \\frac{p}{q}$ <br><br>\n",
    "\n",
    "Then,\n",
    "\n",
    "$$\\frac{p}{q} = \\frac{1}{0!} + \\frac{1}{1!} + \\frac{1}{2!} + . . . + \\frac{1}{q!} $$ <br><br>\n",
    "$$\\frac{p}{q} - \\frac{1}{0!} - . . . - \\frac{1}{q!} = \\frac{1}{(q + 1)!} + . . .  $$ <br><br>\n",
    "$$\\frac{p\\cdot q!}{q} - \\frac{q!}{0!} - . . . - \\frac{q!}{q!} = \\frac{q!}{(q + 1)!} + \\frac{q!}{(q + 2)!} + ... $$ <br><br>\n",
    "$$\\frac{p\\cdot q!}{q} - \\frac{q!}{0!} - . . . - \\frac{q!}{q!} = \\frac{q!}{(q + 1)q!} + \\frac{q!}{(q + 2)(q + 1)q!} + ...$$ <br><br>\n",
    "$$\\frac{p\\cdot q!}{q} - \\frac{q!}{0!} - . . . - \\frac{q!}{q!} = \\frac{1}{q + 1} + \\frac{1}{(q + 2)(q + 1)} + ... $$ <br><br>\n",
    "Is a contradiction. Hence $e$ is irrational.\n",
    "***"
   ]
  },
  {
   "cell_type": "markdown",
   "id": "712c083e",
   "metadata": {},
   "source": [
    "2. Prove Minkowski's Inequality for sums, $\\forall \\ p>1, (a_k, b_k)>0$ &nbsp;: &nbsp; $\\left( \\sum_{k=1}^n |a_k + b_k|^p \\right)^\\frac{1}{p}$ $\\leq$ $\\left( \\sum_{k=1}^n |a_k|^p \\right)^\\frac{1}{p}$ + $\\left( \\sum_{k=1}^n |b_k|^p \\right)^\\frac{1}{p}$\n",
    "\n"
   ]
  },
  {
   "cell_type": "markdown",
   "id": "ba81be01",
   "metadata": {},
   "source": [
    "\n",
    "**Solution:** <br>\n",
    "Proof by Contradiction:\n",
    "\n",
    "Let: <br>\n",
    "$$[ \\left( \\sum_{k=1}^n |a_k + b_k|^p \\right)^{\\frac{1}{p}} > \\left( \\sum_{k=1}^n |a_k|p\\right){\\frac{1}{p}} + \\left( \\sum_{k=1}^n |b_k|p\\right){\\frac{1}{p}} ]$$\n",
    "\n",
    "$$[ \\sum_{k=1}^n |a_k + b_k|^p > \\left( \\sum_{k=1}^n |a_k|^p\\right) + \\left( \\sum_{k=1}^n |b_k|^p\\right) ]$$ <br>\n",
    "\n",
    "Now consider the function $(f(x) = |x|^p)$. By applying Hölder’s Inequality, we have: <br><br>\n",
    "$$[ \\sum_{k=1}^n |a_k + b_k|^p \\leq \\left( \\sum_{k=1}^n |a_k|p\\right){\\frac{1}{p}} \\left( \\sum_{k=1}^n |b_k|p\\right){\\frac{1}{p}} ]$$<br>\n",
    "\n",
    "We have a contradiction since Hölder's Inequality is contradicted by our assumption, which states that the left side of the inequality is greater than the right side. Hence, $$[ \\left( \\sum_{k=1}^n |a_k + b_k|^p \\right)^{\\frac{1}{p}} \\leq \\left( \\sum_{k=1}^n |a_k|p\\right){\\frac{1}{p}} + \\left( \\sum_{k=1}^n |b_k|p\\right){\\frac{1}{p}} ]$$, is True.\n",
    "***"
   ]
  },
  {
   "cell_type": "markdown",
   "id": "acbdb687",
   "metadata": {},
   "source": [
    "3. Prove the triangle inequality $|x+y| \\leq |x| + |y|, \\forall (x,y) \\in \\mathbb{R}$ <br><br>\n",
    "\n",
    "**Solution**:<br><br>\n",
    "Assume $x \\geq 0$ and $y < 0$. <br><br>\n",
    "Then, $|x+y| = -(x+y)$, since $x+y < 0$.<br><br>\n",
    "Also, $|x| = x$ and $|y| = -y$.<br><br>\n",
    "We need to show that $-(x+y) \\leq x - y$.<br><br>\n",
    "Multiplying both sides by $-1$, we get: $x+y \\geq x-(-y) = x+y$, which is always true.<br><br>\n",
    "Since the inequality holds for both cases, we have proved the triangle inequality:\n",
    "$|x+y| \\leq |x| + |y|$ for all $(x,y) \\in \\mathbb{R}$.\n",
    "***"
   ]
  },
  {
   "cell_type": "markdown",
   "id": "111d0d76",
   "metadata": {},
   "source": [
    "4. Prove Sedrakayan's Lemma $\\forall u_i, v_i \\in \\mathbb{R}^+$: <br>\n",
    "$$\\begin{gather} \\frac{(\\Sigma_{i=1}^n u_i)^2}{\\Sigma_{i=1}^n v_i} \\leq \\Sigma_{i=1}^n \\frac{(u_i)^2}{v_i}\\end{gather}$$\n",
    "\n",
    "**Solution**:<br><br>\n",
    "The Cauchy-Schwarz inequality for sequences $\\{a_i\\}$ and $\\{b_i\\}$ states:<br><br>\n",
    "\\begin{equation}\n",
    "   \\left( \\sum_{i=1}^n a_i b_i \\right)^2 \\leq \\left( \\sum_{i=1}^n a_i^2 \\right) \\left( \\sum_{i=1}^n b_i^2 \\right).\n",
    "\\end{equation}<br>\n",
    "\n",
    "Let $a_i = \\frac{u_i}{\\sqrt{v_i}}$ and $b_i = \\sqrt{v_i}$. Then, the left-hand side of the Cauchy-Schwarz inequality becomes:<br>\n",
    "\\begin{equation}\n",
    "   \\left( \\sum_{i=1}^n \\frac{u_i}{\\sqrt{v_i}} \\cdot \\sqrt{v_i} \\right)^2 = \\left( \\sum_{i=1}^n u_i \\right)^2.\n",
    "\\end{equation}<br>\n",
    "\n",
    "The right-hand side of the Cauchy-Schwarz inequality becomes: <br><br>\n",
    "\\begin{equation}\n",
    "   \\left( \\sum_{i=1}^n \\left( \\frac{u_i}{\\sqrt{v_i}} \\right)^2 \\right) \\left( \\sum_{i=1}^n (\\sqrt{v_i})^2 \\right) = \\left( \\sum_{i=1}^n \\frac{u_i^2}{v_i} \\right) \\left( \\sum_{i=1}^n v_i \\right).\n",
    "\\end{equation}<br>\n",
    "\n",
    "By the Cauchy-Schwarz inequality, we have:<br>\n",
    "\\begin{equation}\n",
    "   \\left( \\sum_{i=1}^n u_i \\right)^2 \\leq \\left( \\sum_{i=1}^n \\frac{u_i^2}{v_i} \\right) \\left( \\sum_{i=1}^n v_i \\right).\n",
    "\\end{equation}<br>\n",
    "\n",
    "Dividing both sides of the inequality by $\\sum_{i=1}^n v_i$ gives:<br>\n",
    "\\begin{equation}\n",
    "   \\frac{\\left( \\sum_{i=1}^n u_i \\right)^2}{\\sum_{i=1}^n v_i} \\leq \\sum_{i=1}^n \\frac{u_i^2}{v_i}.\n",
    "\\end{equation}   <br>\n",
    "\n",
    "\n",
    "Therefore, we are able to prove Sedrakayan's Lemma."
   ]
  },
  {
   "cell_type": "markdown",
   "id": "8ec3b3b4",
   "metadata": {},
   "source": [
    "<hr>\n",
    "1. Consider the functions $f(x) = 2x+1$, $g(x)=2y-1$, $j(x) = |f(x)+g(x)|$, and $h(x) = j(x)^2$, show for the following inequality that:\n",
    "\n",
    "\\begin{gather}\n",
    "\\sqrt{|f(x)|^2} \\geq \\sqrt{h(x)} - \\sqrt{|g(x)|^2}, \\forall (x,y) \\in \\mathbb{Z}^+\n",
    "\\end{gather}"
   ]
  },
  {
   "cell_type": "markdown",
   "id": "8aa42913",
   "metadata": {},
   "source": [
    "**solution:** <br><br>\n",
    "With the given functions, we can substitute $f(x)$ and $g(x)$ into $j(x)$:\n",
    "\n",
    "\\begin{equation}\n",
    "    j(x) = |(2x + 1) + (2y - 1)| = |2x + 2y| = 2|x + y|.\n",
    "\\end{equation}\n",
    "\n",
    "With this, we can also find $h(x)$:\n",
    "\n",
    "\\begin{equation}\n",
    "    h(x) = j(x)^2 = (2|x + y|)^2 = 4(x + y)^2.\n",
    "\\end{equation}\n",
    "\n",
    "We can simplify the inequality:\n",
    "\n",
    "\\begin{equation}\n",
    "    \\sqrt{h(x)} = \\sqrt{4(x + y)^2} = 2|x + y|.\n",
    "\\end{equation}\n",
    "\n",
    "\\begin{equation}\n",
    "    \\sqrt{|f(x)|^2} = \\sqrt{(2x + 1)^2} = |2x + 1|\n",
    "\\end{equation}\n",
    "\n",
    "\\begin{equation}\n",
    "    \\sqrt{|g(x)|^2} = \\sqrt{(2y - 1)^2} = |2y - 1|\n",
    "\\end{equation}\n",
    "\n",
    "Now we have:\n",
    "\n",
    "\\begin{equation}\n",
    "    |2x + 1| \\geq 2|x + y| - |2y - 1|\n",
    "\\end{equation}\n",
    "\n",
    "When analyzing the different absolute values in the equation as well as from the given, we can see that:\n",
    "\n",
    "For $( 2x + 1 )$, it's always positive for $( x \\in \\mathbb{Z}^+ )$, hence $( |2x + 1| = 2x + 1 )$.\n",
    "\n",
    "For $( 2y - 1 )$, if $( y \\geq 1 )$, then $( |2y - 1| = 2y - 1)$\n",
    "\n",
    "For $(x + y)$, since $(x,y) \\in \\mathbb{Z}^+$, then $|x + y| = (x + y)$\n",
    "\n",
    "Therefore, the equality can be simplified down to:\n",
    "\n",
    "\\begin{equation}\n",
    "    2x + 1 \\geq 2(x + y) - (2y - 1)\n",
    "\\end{equation}\n",
    "\n",
    "\\begin{equation}\n",
    "    2x + 1 \\geq 2x + 2y - 2y + 1\n",
    "\\end{equation}\n",
    "\n",
    "\\begin{equation}\n",
    "    2x + 1 \\geq 2x + 1\n",
    "\\end{equation}\n",
    "\n",
    "Therefore, the original inequality is proven since $2x + 1 \\geq 2x + 1$ is always true regardless of the value of x."
   ]
  },
  {
   "cell_type": "markdown",
   "id": "6df3e95a",
   "metadata": {},
   "source": [
    "<hr>\n",
    "2. Prove Sedrakayan's Lemma if $u_i, v_i$ are square roots of an even integers:\n",
    "\n",
    "\\begin{gather}\n",
    "\\frac{(\\Sigma_{i=1}^n u_i)^2}{\\Sigma_{i=1}^n v_i}\n",
    "\\leq\n",
    "\\Sigma_{i=1}^n \\frac{(u_i)^2}{v_i}\n",
    "\\end{gather}\n"
   ]
  },
  {
   "cell_type": "markdown",
   "id": "b8284e7f",
   "metadata": {},
   "source": [
    "**solution**:\n",
    "\n",
    "Since $u$ and $v$ are square roots of even integers, we can replace them with $\\sqrt{2a_i}$ and $\\sqrt{2b_i}$ respectively.\n",
    "\n",
    "With this, we can replace the left-hand side of the equation with: <br><br>\n",
    "\n",
    "\\begin{equation}\n",
    "\\frac{\\left( \\sum_{i=1}^n u_i \\right)^2}{\\sum_{i=1}^n v_i} = \\frac{\\left( \\sum_{i=1}^n \\sqrt{2a_i} \\right)^2}{\\sum_{i=1}^n \\sqrt{2b_i}}.\n",
    "\\end{equation} <br>\n",
    "\n",
    "Simplifying the numerator and the denominator: <br><br>\n",
    "\n",
    "\\begin{equation}\n",
    "\\frac{\\left( \\sum_{i=1}^n \\sqrt{2a_i} \\right)^2}{\\sum_{i=1}^n \\sqrt{2b_i}} = \\frac{2\\left( \\sum_{i=1}^n \\sqrt{a_i} \\right)^2}{2\\sum_{i=1}^n \\sqrt{b_i}} = \\frac{\\left( \\sum_{i=1}^n \\sqrt{a_i} \\right)^2}{\\sum_{i=1}^n \\sqrt{b_i}}.\n",
    "\\end{equation} <br>\n",
    "\n",
    "Now, compute the right-hand side: <br><br>\n",
    "\n",
    "\\begin{equation}\n",
    "\\sum_{i=1}^n \\frac{u_i^2}{v_i} = \\sum_{i=1}^n \\frac{(\\sqrt{2a_i})^2}{\\sqrt{2b_i}} = \\sum_{i=1}^n \\frac{2a_i}{\\sqrt{2b_i}} = \\sum_{i=1}^n \\frac{2a_i}{\\sqrt{2}\\sqrt{b_i}} = \\sum_{i=1}^n \\frac{2a_i}{\\sqrt{2b_i}} = \\sqrt{2} \\sum_{i=1}^n \\frac{a_i}{\\sqrt{b_i}}.\n",
    "\\end{equation} <br>\n",
    "\n",
    "So, the inequality becomes: <br><br>\n",
    "\n",
    "\\begin{equation}\n",
    "\\frac{\\left( \\sum_{i=1}^n \\sqrt{a_i} \\right)^2}{\\sum_{i=1}^n \\sqrt{b_i}} \\leq \\sqrt{2} \\sum_{i=1}^n \\frac{a_i}{\\sqrt{b_i}}.\n",
    "\\end{equation} <br>\n",
    "\n",
    "We can now analyze and prove this inequality utilizing the Cauchy-Schwarz inequality.\n",
    "\n",
    "By the Cauchy-Schwarz inequality applied to the sequences $( \\sqrt{a_i} )$ and $( \\frac{1}{\\sqrt{b_i}} )$: <br><br>\n",
    "\n",
    "\\begin{equation}\n",
    "\\left( \\sum_{i=1}^n \\sqrt{a_i} \\cdot \\frac{1}{\\sqrt{b_i}} \\right)^2 \\leq \\left( \\sum_{i=1}^n (\\sqrt{a_i})^2 \\right) \\left( \\sum_{i=1}^n \\left( \\frac{1}{\\sqrt{b_i}} \\right)^2 \\right).\n",
    "\\end{equation} <br>\n",
    "\n",
    "Simplify the terms: <br><br>\n",
    "\n",
    "\\begin{equation}\n",
    "\\left( \\sum_{i=1}^n \\frac{\\sqrt{a_i}}{\\sqrt{b_i}} \\right)^2 \\leq \\left( \\sum_{i=1}^n a_i \\right) \\left( \\sum_{i=1}^n \\frac{1}{b_i} \\right).\n",
    "\\end{equation} <br>\n",
    "\n",
    "To apply this to our problem, we can rewrite the original left-hand side as follows: <br><br>\n",
    "\n",
    "\\begin{equation}\n",
    "\\frac{\\left( \\sum_{i=1}^n \\sqrt{a_i} \\right)^2}{\\sum_{i=1}^n \\sqrt{b_i}} = \\frac{\\left( \\sum_{i=1}^n \\sqrt{a_i} \\cdot \\sqrt{b_i} \\cdot \\frac{1}{\\sqrt{b_i}} \\right)^2}{\\sum_{i=1}^n \\sqrt{b_i}}.\n",
    "\\end{equation} <br>\n",
    "\n",
    "Using the Cauchy-Schwarz inequality result: <br><br>\n",
    "\n",
    "\\begin{equation}\n",
    "\\left( \\sum_{i=1}^n \\sqrt{a_i} \\cdot \\frac{1}{\\sqrt{b_i}} \\right)^2 \\leq \\left( \\sum_{i=1}^n a_i \\right) \\left( \\sum_{i=1}^n \\frac{1}{b_i} \\right).\n",
    "\\end{equation} <br>\n",
    "\n",
    "Thus: <br><br>\n",
    "\n",
    "\\begin{equation}\n",
    "\\frac{\\left( \\sum_{i=1}^n \\sqrt{a_i} \\right)^2}{\\sum_{i=1}^n \\sqrt{b_i}} \\leq \\frac{\\left( \\sum_{i=1}^n a_i \\right)}{\\sum_{i=1}^n \\frac{1}{b_i}}.\n",
    "\\end{equation} <br>\n",
    "\n",
    "Therefore, we have shown: <br><br>\n",
    "\n",
    "\\begin{equation}\n",
    "\\frac{\\left( \\sum_{i=1}^n u_i \\right)^2}{\\sum_{i=1}^n v_i} \\leq \\sum_{i=1}^n \\frac{u_i^2}{v_i}.\n",
    "\\end{equation}"
   ]
  },
  {
   "cell_type": "code",
   "execution_count": null,
   "id": "68e2bb2b",
   "metadata": {},
   "outputs": [],
   "source": []
  }
 ],
 "metadata": {
  "kernelspec": {
   "display_name": "Python 3 (ipykernel)",
   "language": "python",
   "name": "python3"
  },
  "language_info": {
   "codemirror_mode": {
    "name": "ipython",
    "version": 3
   },
   "file_extension": ".py",
   "mimetype": "text/x-python",
   "name": "python",
   "nbconvert_exporter": "python",
   "pygments_lexer": "ipython3",
   "version": "3.11.7"
  }
 },
 "nbformat": 4,
 "nbformat_minor": 5
}
